Work towards cake_ag32_next

compiler/bootstrap/compilation/ag32/32/proofs/ag32BootstrapProofScript.sml
@@ -1,5 +1,7 @@
 open preamble
-     semanticsPropsTheory backendProofTheory ag32_configProofTheory
+     semanticsPropsTheory backendProofTheory
+     ag32_configProofTheory ag32_machine_configTheory
+     ag32_memoryProofTheory ag32_basis_ffiProofTheory
      compiler32ProgTheory ag32BootstrapTheory
 
 val _ = new_theory"ag32BootstrapProof";
@@ -22,6 +24,48 @@ val with_clos_conf_simp = prove(
   fs [mc_init_ok_def,FUN_EQ_THM,backend_config_ok_def]
   \\ rw [] \\ eq_tac \\ rw [] \\ EVAL_TAC);
 
+val ffi_names =
+  ``config.ffi_names``
+  |> (REWRITE_CONV[ag32BootstrapTheory.config_def] THENC EVAL)
+
+val LENGTH_code =
+  ``LENGTH code``
+  |> (REWRITE_CONV[ag32BootstrapTheory.code_def] THENC listLib.LENGTH_CONV)
+
+val LENGTH_data =
+  ``LENGTH data``
+  |> (REWRITE_CONV[ag32BootstrapTheory.data_def] THENC listLib.LENGTH_CONV)
+
+val _ = overload_on("cake_machine_config",
+    ``ag32_machine_config (THE config.ffi_names) (LENGTH code) (LENGTH data)``);
+
+val target_state_rel_cake_start_asm_state = Q.store_thm("target_state_rel_cake_start_asm_state",
+  `SUM (MAP strlen cl) + LENGTH cl ≤ cline_size ∧
+   LENGTH inp ≤ stdin_size ∧
+   is_ag32_init_state (init_memory code data (THE config.ffi_names) (cl,inp)) ms ⇒
+   ∃n. target_state_rel ag32_target (init_asm_state code data (THE config.ffi_names) (cl,inp)) (FUNPOW Next n ms) ∧
+       ((FUNPOW Next n ms).io_events = ms.io_events) ∧
+       (∀x. x ∉ (ag32_startup_addresses) ⇒
+         ((FUNPOW Next n ms).MEM x = ms.MEM x))`,
+  strip_tac
+  \\ drule (GEN_ALL init_asm_state_RTC_asm_step)
+  \\ disch_then drule
+  \\ simp_tac std_ss []
+  \\ disch_then(qspecl_then[`code`,`data`,`THE config.ffi_names`]mp_tac)
+  \\ impl_tac >- ( EVAL_TAC>> fs[ffi_names,LENGTH_data,LENGTH_code])
+  \\ strip_tac
+  \\ drule (GEN_ALL target_state_rel_ag32_init)
+  \\ rveq
+  \\ qmatch_goalsub_abbrev_tac`_ ∉ md`
+  \\ disch_then(qspec_then`md`assume_tac)
+  \\ drule (GEN_ALL RTC_asm_step_ag32_target_state_rel_io_events)
+  \\ simp[EVAL``(ag32_init_asm_state m md).mem_domain``]);
+
+val cake_startup_clock_def =
+  new_specification("cake_startup_clock_def",["cake_startup_clock"],
+  GEN_ALL (Q.SPEC`ms0`(Q.GEN`ms`target_state_rel_cake_start_asm_state))
+  |> SIMP_RULE bool_ss [GSYM RIGHT_EXISTS_IMP_THM,SKOLEM_THM]);
+
 val compile_correct_applied =
   MATCH_MP compile_correct cake_compiled
   |> SIMP_RULE(srw_ss())[LET_THM,ml_progTheory.init_state_env_thm,GSYM AND_IMP_INTRO,
@@ -32,14 +76,172 @@ val compile_correct_applied =
   |> REWRITE_RULE[Once (GSYM AND_IMP_INTRO)]
   |> C MATCH_MP (CONJ(UNDISCH ag32_machine_config_ok)(UNDISCH ag32_init_ok))
   |> DISCH(#1(dest_imp(concl ag32_init_ok)))
-  |> REWRITE_RULE[AND_IMP_INTRO]
+  |> C MATCH_MP is_ag32_machine_config_ag32_machine_config
+  |> Q.GEN`cbspace` |> Q.SPEC`0`
+  |> Q.GEN`data_sp` |> Q.SPEC`0`
 
-val cake_compiled_thm =
-  CONJ compile_correct_applied cake_output
+val cake_installed = Q.store_thm("cake_installed",
+  `SUM (MAP strlen cl) + LENGTH cl ≤ cline_size ∧
+   LENGTH inp ≤ stdin_size ∧
+   is_ag32_init_state (init_memory code data (THE config.ffi_names) (cl,inp)) ms0 ⇒
+   installed code 0 data 0 config.ffi_names (basis_ffi cl fs)
+     (heap_regs ag32_backend_config.stack_conf.reg_names)
+     (cake_machine_config) (FUNPOW Next (cake_startup_clock ms0 inp cl) ms0)`,
+  rewrite_tac[ffi_names, THE_DEF]
+  \\ strip_tac
+  \\ irule ag32_installed
+  \\ drule cake_startup_clock_def
+  \\ disch_then drule
+  \\ rewrite_tac[ffi_names, THE_DEF]
+  \\ disch_then drule
+  \\ strip_tac
+  \\ simp[]
+  \\ conj_tac >- (simp[LENGTH_code] \\ EVAL_TAC)
+  \\ conj_tac >- (simp[LENGTH_code, LENGTH_data] \\ EVAL_TAC)
+  \\ conj_tac >- (
+    conj_tac >- cheat (* need to support empty ffi (or turn it off) *)
+    \\ EVAL_TAC)
+  \\ asm_exists_tac \\ simp[]);
+
+val cake_machine_sem =
+  compile_correct_applied
+  |> C MATCH_MP (UNDISCH cake_installed)
   |> DISCH_ALL
-  |> check_thm
-  |> curry save_thm "cake_compiled_thm";
+  |> curry save_thm "cake_machine_sem";
 
-(* TODO: compose this with a correctness theorem for compiler_x32? *)
+(* TODO: move *)
+val get_stdin_stdin_fs = Q.store_thm("get_stdin_stdin_fs[simp]",
+  `get_stdin (stdin_fs inp) = inp`,
+  EVAL_TAC
+  \\ SELECT_ELIM_TAC
+  \\ simp[EXISTS_PROD, FORALL_PROD]);
+
+val inFS_fname_fastForwardFD = Q.store_thm("inFS_fname_fastForwardFD[simp]",
+  `inFS_fname (fastForwardFD fs fd) fnm ⇔ inFS_fname fs fnm`,
+  rw[fsFFIPropsTheory.inFS_fname_def]);
+
+val File_NOTIN_stdin_fs = Q.store_thm("File_NOTIN_stdin_fs[simp]",
+  `∀nm. ¬ inFS_fname (stdin_fs inp) (File nm)`,
+  rw[stdin_fs_def,fsFFIPropsTheory.inFS_fname_def]);
+
+val ALOOKUP_fastForwardFD_infds_neq = Q.store_thm("ALOOKUP_fastForwardFD_infds_neq",
+  `fd ≠ fd' ⇒ (ALOOKUP (fastForwardFD fs fd).infds fd' = ALOOKUP fs.infds fd')`,
+  rw[fsFFIPropsTheory.fastForwardFD_def]
+  \\ Cases_on`ALOOKUP fs.infds fd` \\ simp[libTheory.the_def]
+  \\ pairarg_tac \\ simp[]
+  \\ Cases_on`ALOOKUP fs.files fnm` \\ simp[libTheory.the_def]
+  \\ simp[ALIST_FUPDKEY_ALOOKUP]
+  \\ CASE_TAC);
+
+val FST_ALOOKUP_fastForwardFD_infds = Q.store_thm("FST_ALOOKUP_fastForwardFD_infds",
+  `OPTION_MAP FST (ALOOKUP (fastForwardFD fs fd).infds fd') = OPTION_MAP FST (ALOOKUP fs.infds fd')`,
+  rw[fsFFIPropsTheory.fastForwardFD_def]
+  \\ Cases_on`ALOOKUP fs.infds fd` \\ simp[libTheory.the_def]
+  \\ pairarg_tac \\ simp[]
+  \\ Cases_on`ALOOKUP fs.files fnm` \\ simp[libTheory.the_def]
+  \\ simp[ALIST_FUPDKEY_ALOOKUP]
+  \\ CASE_TAC \\ simp[]
+  \\ CASE_TAC \\ simp[]);
+(* -- *)
+
+val cake_extract_writes = Q.store_thm("cake_extract_writes",
+  `wfcl cl ⇒
+   let events = MAP get_output_io_event (cake_io_events cl (stdin_fs inp)) in
+   let out = extract_writes 1 events in
+   let err = extract_writes 2 events in
+   if has_version_flag (TL cl) then
+     (out = explode current_build_info_str) ∧ (err = "")
+   else
+     let (cout, cerr) = compile_32 (TL cl) inp in
+     (out = explode (concat (append cout))) ∧
+     (err = explode cerr)`,
+  strip_tac
+  \\ drule(GEN_ALL(DISCH_ALL cake_output))
+  \\ disch_then(qspec_then`stdin_fs inp`mp_tac)
+  \\ simp[wfFS_stdin_fs, STD_streams_stdin_fs]
+  \\ simp[compilerTheory.full_compile_32_def]
+  \\ pairarg_tac \\ simp[]
+  \\ IF_CASES_TAC \\ fs[]
+  >- (
+    simp[TextIOProofTheory.add_stdo_def]
+    \\ SELECT_ELIM_TAC
+    \\ simp[TextIOProofTheory.stdo_def]
+    \\ conj_tac
+    >- (
+      simp[stdin_fs_def]
+      \\ qexists_tac`implode""`
+      \\ simp[] )
+    \\ simp[Once stdin_fs_def, ALIST_FUPDKEY_def]
+    \\ Cases \\ simp[] \\ strip_tac \\ rveq
+    \\ pop_assum mp_tac
+    \\ simp[TextIOProofTheory.up_stdo_def]
+    \\ simp[fsFFITheory.fsupdate_def]
+    \\ simp[stdin_fs_def]
+    \\ rw[]
+    \\ (
+      drule (GEN_ALL extract_fs_extract_writes)
+      \\ simp[ALIST_FUPDKEY_ALOOKUP]
+      \\ disch_then match_mp_tac
+      \\ rw[fsFFIPropsTheory.inFS_fname_def]
+      >- (fs[CaseEq"option",CaseEq"bool"] \\ rveq \\ fs[])
+      >- (
+        pop_assum mp_tac
+        \\ rw[] \\ fs[] \\ rw[]
+        \\ pop_assum mp_tac \\ rw[])
+      >- ( rw[] \\ rw[OPTREL_def])))
+  \\ simp[TextIOProofTheory.add_stdout_fastForwardFD, STD_streams_stdin_fs]
+  \\ DEP_REWRITE_TAC[TextIOProofTheory.add_stderr_fastForwardFD]
+  \\ simp[TextIOProofTheory.STD_streams_add_stdout, STD_streams_stdin_fs]
+  \\ strip_tac
+  \\ drule (GEN_ALL extract_fs_extract_writes)
+  \\ simp[]
+  \\ simp[Once stdin_fs_def]
+  \\ strip_tac
+  \\ conj_tac
+  >- (
+    first_x_assum irule
+    \\ simp[ALOOKUP_fastForwardFD_infds_neq]
+    \\ cheat (* prove more lemmas, and/or similar to previously *))
+  \\ first_x_assum irule
+  \\ simp[ALOOKUP_fastForwardFD_infds_neq]
+  \\ cheat (* more of the same *));
+
+val cake_ag32_next = Q.store_thm("cake_ag32_next",
+  `SUM (MAP strlen cl) + LENGTH cl ≤ cline_size ∧ wfcl cl ∧
+   LENGTH inp ≤ stdin_size ∧
+   is_ag32_init_state (init_memory code data (THE config.ffi_names) (cl,inp)) ms0
+  ⇒
+   ∃k1. ∀k. k1 ≤ k ⇒
+     let ms = FUNPOW Next k ms0 in
+     let outs = MAP (get_ag32_io_event) ms.io_events in
+       (ms.PC = (cake_machine_config).halt_pc) ∧
+       outs ≼ MAP get_output_io_event (cake_io_events cl (stdin_fs inp)) ∧
+       ((ms.R (n2w (cake_machine_config).ptr_reg) = 0w) ⇒
+        (outs = MAP get_output_io_event (cake_io_events cl (stdin_fs inp))))`,
+  strip_tac
+  \\ drule (GEN_ALL cake_machine_sem)
+  \\ disch_then drule
+  \\ disch_then drule
+  \\ disch_then(qspec_then`stdin_fs inp`mp_tac)
+  \\ impl_tac >- fs[STD_streams_stdin_fs, wfFS_stdin_fs]
+  \\ strip_tac
+  \\ irule ag32_next
+  \\ conj_tac >- simp[ffi_names]
+  \\ conj_tac >- (simp[ffi_names, LENGTH_code, LENGTH_data] \\ EVAL_TAC)
+  \\ conj_tac >- (simp[ffi_names]
+    conj_tac >- cheat (* need to support empty ffi (or turn it off) *)
+    \\ EVAL_TAC)
+  \\ goal_assum(first_assum o mp_then Any mp_tac)
+  \\ goal_assum(first_assum o mp_then Any mp_tac)
+  \\ goal_assum(first_assum o mp_then Any mp_tac)
+  \\ goal_assum(first_assum o mp_then Any mp_tac)
+  \\ goal_assum(first_assum o mp_then Any mp_tac)
+  \\ drule cake_startup_clock_def
+  \\ disch_then drule
+  \\ disch_then drule
+  \\ strip_tac
+  \\ goal_assum(first_assum o mp_then Any mp_tac)
+  \\ goal_assum(first_assum o mp_then Any mp_tac)
+  \\ metis_tac[]);
 
 val _ = export_theory();
